@prefix : <http://www.semanticweb.org/usuario/ontologies/2025/3/Turismo_Inteligente_Recomendaciones#> .
@prefix owl: <http://www.w3.org/2002/07/owl#> .
@prefix rdf: <http://www.w3.org/1999/02/22-rdf-syntax-ns#> .
@prefix xml: <http://www.w3.org/XML/1998/namespace> .
@prefix xsd: <http://www.w3.org/2001/XMLSchema#> .
@prefix rdfs: <http://www.w3.org/2000/01/rdf-schema#> .
@base <http://www.semanticweb.org/usuario/ontologies/2025/3/Turismo_Inteligente_Recomendaciones#> .

<http://www.semanticweb.org/usuario/ontologies/2025/3/Turismo_Inteligente_Recomendaciones> rdf:type owl:Ontology .

#################################################################
#    Annotation properties
#################################################################

###  http://swrl.stanford.edu/ontologies/3.3/swrla.owl#isRuleEnabled
<http://swrl.stanford.edu/ontologies/3.3/swrla.owl#isRuleEnabled> rdf:type owl:AnnotationProperty .


###  http://www.w3.org/2000/01/rdf-schema#sameAs
rdfs:sameAs rdf:type owl:AnnotationProperty .


#################################################################
#    Datatypes
#################################################################

###  http://www.w3.org/2001/XMLSchema#date
xsd:date rdf:type rdfs:Datatype .


#################################################################
#    Object Properties
#################################################################

###  http://www.semanticweb.org/usuario/ontologies/2025/3/Turismo_Inteligente_Recomendaciones#hasAttraction
:hasAttraction rdf:type owl:ObjectProperty ;
               rdfs:domain :City ;
               rdfs:range :Attraction .


###  http://www.semanticweb.org/usuario/ontologies/2025/3/Turismo_Inteligente_Recomendaciones#hasEvent
:hasEvent rdf:type owl:ObjectProperty ;
          rdfs:domain :City ;
          rdfs:range :Event .


###  http://www.semanticweb.org/usuario/ontologies/2025/3/Turismo_Inteligente_Recomendaciones#hasHotel
:hasHotel rdf:type owl:ObjectProperty ;
          rdfs:domain :City ;
          rdfs:range :Hotel .


###  http://www.semanticweb.org/usuario/ontologies/2025/3/Turismo_Inteligente_Recomendaciones#hasPrice
:hasPrice rdf:type owl:ObjectProperty ;
          rdfs:domain [ rdf:type owl:Class ;
                        owl:unionOf ( :Hotel
                                      :Restaurant
                                      :Transport
                                    )
                      ] ;
          rdfs:range :Price .


###  http://www.semanticweb.org/usuario/ontologies/2025/3/Turismo_Inteligente_Recomendaciones#hasRating
:hasRating rdf:type owl:ObjectProperty ;
           rdfs:domain [ rdf:type owl:Class ;
                         owl:unionOf ( :Attraction
                                       :Hotel
                                       :Restaurant
                                     )
                       ] ;
           rdfs:range :Rating .


###  http://www.semanticweb.org/usuario/ontologies/2025/3/Turismo_Inteligente_Recomendaciones#hasRestaurant
:hasRestaurant rdf:type owl:ObjectProperty ;
               rdfs:domain :City ;
               rdfs:range :Restaurant .


###  http://www.semanticweb.org/usuario/ontologies/2025/3/Turismo_Inteligente_Recomendaciones#hasStars
:hasStars rdf:type owl:ObjectProperty ;
          rdfs:domain :Hotel ;
          rdfs:range :HotelStars .


###  http://www.semanticweb.org/usuario/ontologies/2025/3/Turismo_Inteligente_Recomendaciones#hasTransport
:hasTransport rdf:type owl:ObjectProperty ;
              rdfs:domain :City ;
              rdfs:range :Transport .


###  http://www.semanticweb.org/usuario/ontologies/2025/3/Turismo_Inteligente_Recomendaciones#isLocatedIn
:isLocatedIn rdf:type owl:ObjectProperty ;
             rdfs:domain [ rdf:type owl:Class ;
                           owl:unionOf ( :Attraction
                                         :Event
                                         :Hotel
                                         :Restaurant
                                         :Transport
                                       )
                         ] ;
             rdfs:range :City .


#################################################################
#    Data properties
#################################################################

###  http://www.semanticweb.org/usuario/ontologies/2025/3/Turismo_Inteligente_Recomendaciones#attraction_id
:attraction_id rdf:type owl:DatatypeProperty ;
               rdfs:domain :Attraction ;
               rdfs:range xsd:integer .


###  http://www.semanticweb.org/usuario/ontologies/2025/3/Turismo_Inteligente_Recomendaciones#avg_price
:avg_price rdf:type owl:DatatypeProperty ;
           rdfs:domain :Restaurant ;
           rdfs:range xsd:decimal .


###  http://www.semanticweb.org/usuario/ontologies/2025/3/Turismo_Inteligente_Recomendaciones#event_id
:event_id rdf:type owl:DatatypeProperty ;
          rdfs:domain :Event ;
          rdfs:range xsd:integer .


###  http://www.semanticweb.org/usuario/ontologies/2025/3/Turismo_Inteligente_Recomendaciones#hasCityId
:hasCityId rdf:type owl:DatatypeProperty ;
           rdfs:domain :City ;
           rdfs:range xsd:integer .


###  http://www.semanticweb.org/usuario/ontologies/2025/3/Turismo_Inteligente_Recomendaciones#hasCoordinates
:hasCoordinates rdf:type owl:DatatypeProperty ;
                rdfs:domain :City ;
                rdfs:range xsd:string .


###  http://www.semanticweb.org/usuario/ontologies/2025/3/Turismo_Inteligente_Recomendaciones#hasDate
:hasDate rdf:type owl:DatatypeProperty ;
         rdfs:domain :Event ;
         rdfs:range xsd:date .


###  http://www.semanticweb.org/usuario/ontologies/2025/3/Turismo_Inteligente_Recomendaciones#hotel_id
:hotel_id rdf:type owl:DatatypeProperty ;
          rdfs:domain :Hotel ;
          rdfs:range xsd:integer .


###  http://www.semanticweb.org/usuario/ontologies/2025/3/Turismo_Inteligente_Recomendaciones#name
:name rdf:type owl:DatatypeProperty ;
      rdfs:domain [ rdf:type owl:Class ;
                    owl:unionOf ( :Attraction
                                  :City
                                  :Event
                                  :Hotel
                                  :Restaurant
                                )
                  ] ;
      rdfs:range xsd:string .


###  http://www.semanticweb.org/usuario/ontologies/2025/3/Turismo_Inteligente_Recomendaciones#price_per_night
:price_per_night rdf:type owl:DatatypeProperty ;
                 rdfs:domain :Hotel ;
                 rdfs:range xsd:integer .


###  http://www.semanticweb.org/usuario/ontologies/2025/3/Turismo_Inteligente_Recomendaciones#restaurant_id
:restaurant_id rdf:type owl:DatatypeProperty ;
               rdfs:domain :Restaurant ;
               rdfs:range xsd:integer .


###  http://www.semanticweb.org/usuario/ontologies/2025/3/Turismo_Inteligente_Recomendaciones#transport_id
:transport_id rdf:type owl:DatatypeProperty ;
              rdfs:domain :Transport ;
              rdfs:range xsd:integer .


#################################################################
#    Classes
#################################################################

###  http://www.semanticweb.org/usuario/ontologies/2025/3/Turismo_Inteligente_Recomendaciones#AndalusianRestaurant
:AndalusianRestaurant rdf:type owl:Class ;
                      rdfs:subClassOf :Restaurant ;
                      rdfs:comment "A restaurant specializing in Andalusian cuisine, characterized by rich Mediterranean flavors and regional Spanish dishes"@en ;
                      rdfs:label "Andalusian Restaurant"@en .


###  http://www.semanticweb.org/usuario/ontologies/2025/3/Turismo_Inteligente_Recomendaciones#Attraction
:Attraction rdf:type owl:Class ;
            rdfs:subClassOf [ rdf:type owl:Restriction ;
                              owl:onProperty :isLocatedIn ;
                              owl:qualifiedCardinality "1"^^xsd:nonNegativeInteger ;
                              owl:onClass :City
                            ] ;
            rdfs:comment "An attraction is a place or point of interest that draws visitors for its cultural, historical, natural, or recreational value."@en ;
            rdfs:label "Attraction"@en .


###  http://www.semanticweb.org/usuario/ontologies/2025/3/Turismo_Inteligente_Recomendaciones#Beach
:Beach rdf:type owl:Class ;
       rdfs:subClassOf :Attraction ;
       owl:disjointWith :CulturalAttraction ,
                        :Monument ,
                        :Museum ,
                        :Park ;
       rdfs:comment "A beach is a tourist attracion by the seaside."@en ;
       rdfs:label "Beach"@en ;
       rdfs:sameAs "https://dbpedia.org/page/Beach" .


###  http://www.semanticweb.org/usuario/ontologies/2025/3/Turismo_Inteligente_Recomendaciones#BeachHotel
:BeachHotel rdf:type owl:Class ;
            rdfs:subClassOf :Hotel ;
            rdfs:comment "A beach hotel is a hotel located near or with direct access to the beach, catering primarily to vacationers."@en ;
            rdfs:label "BeachHotel"@en .


###  http://www.semanticweb.org/usuario/ontologies/2025/3/Turismo_Inteligente_Recomendaciones#Bicicle
:Bicicle rdf:type owl:Class ;
         rdfs:subClassOf :Transport ;
         rdfs:comment "A two-wheeled vehicle powered by pedaling, commonly used for personal transport and recreation."@en ;
         rdfs:label "Bycicle"@en .


###  http://www.semanticweb.org/usuario/ontologies/2025/3/Turismo_Inteligente_Recomendaciones#Bus
:Bus rdf:type owl:Class ;
     rdfs:subClassOf :Transport ;
     rdfs:comment "A road vehicle designed to carry multiple passengers along predetermined routes"@en ;
     rdfs:label "Bus"@en .


###  http://www.semanticweb.org/usuario/ontologies/2025/3/Turismo_Inteligente_Recomendaciones#BusinessHotel
:BusinessHotel rdf:type owl:Class ;
               rdfs:subClassOf :Hotel ;
               rdfs:comment "A business hotel is a hotel designed to accommodate business travelers, often offering services such as conference rooms, Wi-Fi, and business centers."@en ;
               rdfs:label "BusinessHotel"@en .


###  http://www.semanticweb.org/usuario/ontologies/2025/3/Turismo_Inteligente_Recomendaciones#City
:City rdf:type owl:Class ;
      rdfs:subClassOf [ rdf:type owl:Restriction ;
                        owl:onProperty :hasCoordinates ;
                        owl:someValuesFrom xsd:string
                      ] ;
      rdfs:comment "A city is a place where a community of people live"@en ;
      rdfs:label "City"@en ;
      rdfs:sameAs "https://dbpedia.org/page/City" .


###  http://www.semanticweb.org/usuario/ontologies/2025/3/Turismo_Inteligente_Recomendaciones#CountrysideHotel
:CountrysideHotel rdf:type owl:Class ;
                  rdfs:subClassOf :Hotel ;
                  rdfs:comment "A countryside hote is a hotel situated in rural or natural settings, ideal for guests seeking relaxation or eco-tourism experiences."@en ;
                  rdfs:label "CountrysideHotel"@en .


###  http://www.semanticweb.org/usuario/ontologies/2025/3/Turismo_Inteligente_Recomendaciones#CulinaryEvent
:CulinaryEvent rdf:type owl:Class ;
               rdfs:subClassOf :Event ;
               rdfs:comment "Culinary event is an event related to gastronomy, where food, beverages, or culinary traditions are showcased, promoted, or celebrated."@en ;
               rdfs:label "Culinary event"@en .


###  http://www.semanticweb.org/usuario/ontologies/2025/3/Turismo_Inteligente_Recomendaciones#CulturalAttraction
:CulturalAttraction rdf:type owl:Class ;
                    rdfs:subClassOf :Attraction ;
                    rdfs:comment "A cultural attraction is a miscellaneous attraction of any sort"@en ;
                    rdfs:label "Cultural attraction"@en .


###  http://www.semanticweb.org/usuario/ontologies/2025/3/Turismo_Inteligente_Recomendaciones#CulturalEvent
:CulturalEvent rdf:type owl:Class ;
               rdfs:subClassOf :Event ;
               rdfs:comment "A cultural event is an organized activity aimed at promoting, celebrating, or preserving artistic or traditional expressions of a community or region."@en ;
               rdfs:label "CulturalEvent"@en .


###  http://www.semanticweb.org/usuario/ontologies/2025/3/Turismo_Inteligente_Recomendaciones#Event
:Event rdf:type owl:Class ;
       rdfs:subClassOf [ rdf:type owl:Restriction ;
                         owl:onProperty :isLocatedIn ;
                         owl:qualifiedCardinality "1"^^xsd:nonNegativeInteger ;
                         owl:onClass :City
                       ] ;
       rdfs:comment "An event is a scheduled public or private activity organized for entertainment, cultural, educational, or promotional purposes."@en ;
       rdfs:label "Event"@en .


###  http://www.semanticweb.org/usuario/ontologies/2025/3/Turismo_Inteligente_Recomendaciones#HighRating
:HighRating rdf:type owl:Class ;
            rdfs:subClassOf :Rating ;
            rdfs:comment "Denotes a rating that indicates a very positive evaluation, usually close to the maximum score."@en ;
            rdfs:label "High Rating"@en .


###  http://www.semanticweb.org/usuario/ontologies/2025/3/Turismo_Inteligente_Recomendaciones#Hotel
:Hotel rdf:type owl:Class ;
       rdfs:subClassOf [ rdf:type owl:Restriction ;
                         owl:onProperty :hasStars ;
                         owl:qualifiedCardinality "1"^^xsd:nonNegativeInteger ;
                         owl:onClass :HotelStars
                       ] ,
                       [ rdf:type owl:Restriction ;
                         owl:onProperty :isLocatedIn ;
                         owl:qualifiedCardinality "1"^^xsd:nonNegativeInteger ;
                         owl:onClass :City
                       ] ;
       rdfs:comment "An hotel is an establishment that provides lodging services to travelers and tourists, typically including amenities like meals, cleaning, and reception."@en ;
       rdfs:label "Hotel"@en ;
       rdfs:sameAs "https://dbpedia.org/page/Hotel" .


###  http://www.semanticweb.org/usuario/ontologies/2025/3/Turismo_Inteligente_Recomendaciones#HotelStars
:HotelStars rdf:type owl:Class ;
            rdfs:comment "Represents the official star classification awarded to hotels based on quality and service standards"@en ;
            rdfs:label "HotelStars"@en .


###  http://www.semanticweb.org/usuario/ontologies/2025/3/Turismo_Inteligente_Recomendaciones#ItalianRestaurant
:ItalianRestaurant rdf:type owl:Class ;
                   rdfs:subClassOf :Restaurant ;
                   rdfs:comment "A restaurant specializing in Italian cuisine, known for dishes such as pasta, pizza, and regional Italian specialties"@en ;
                   rdfs:label "Italian Restaurant"@en .


###  http://www.semanticweb.org/usuario/ontologies/2025/3/Turismo_Inteligente_Recomendaciones#JapaneseRestaurant
:JapaneseRestaurant rdf:type owl:Class ;
                    rdfs:subClassOf :Restaurant ;
                    rdfs:comment "A restaurant specializing in Japanese cuisine, including sushi, sashimi, ramen, and traditional Japanese dishes."@en ;
                    rdfs:label "Japanese Restaurant"@en .


###  http://www.semanticweb.org/usuario/ontologies/2025/3/Turismo_Inteligente_Recomendaciones#LowRating
:LowRating rdf:type owl:Class ;
           rdfs:subClassOf :Rating ;
           rdfs:comment "Denotes a rating that reflects a poor evaluation or low level of satisfaction"@en ;
           rdfs:label "Low Rating"@en .


###  http://www.semanticweb.org/usuario/ontologies/2025/3/Turismo_Inteligente_Recomendaciones#LuxuryHotel
:LuxuryHotel rdf:type owl:Class ;
             rdfs:subClassOf :Hotel ;
             rdfs:comment "A luxury hotel is a high-end hotel offering premium services, accommodations, and exclusive amenities to its guests."@en ;
             rdfs:label "LuxuryHotel"@en .


###  http://www.semanticweb.org/usuario/ontologies/2025/3/Turismo_Inteligente_Recomendaciones#MediterraneanRestaurant
:MediterraneanRestaurant rdf:type owl:Class ;
                         rdfs:subClassOf :Restaurant ;
                         rdfs:comment "A restaurant offering dishes inspired by Mediterranean culinary traditions, emphasizing fresh ingredients, olive oil, and healthy recipes."@en ;
                         rdfs:label "Mediterranean Restaurant"@en .


###  http://www.semanticweb.org/usuario/ontologies/2025/3/Turismo_Inteligente_Recomendaciones#MediumRating
:MediumRating rdf:type owl:Class ;
              rdfs:subClassOf :Rating ;
              rdfs:comment "Denotes an average rating, representing a moderate level of satisfaction or quality."@en ;
              rdfs:label "Medium Rating"@en .


###  http://www.semanticweb.org/usuario/ontologies/2025/3/Turismo_Inteligente_Recomendaciones#Metro
:Metro rdf:type owl:Class ;
       rdfs:subClassOf :Transport .


###  http://www.semanticweb.org/usuario/ontologies/2025/3/Turismo_Inteligente_Recomendaciones#MexicanRestaurant
:MexicanRestaurant rdf:type owl:Class ;
                   rdfs:subClassOf :Restaurant ;
                   rdfs:comment "A restaurant specializing in Mexican cuisine, featuring dishes like tacos, enchiladas, and a variety of spicy flavors."@en ;
                   rdfs:label "Mexican Restaurant"@en .


###  http://www.semanticweb.org/usuario/ontologies/2025/3/Turismo_Inteligente_Recomendaciones#Monument
:Monument rdf:type owl:Class ;
          rdfs:subClassOf :Attraction ;
          rdfs:comment "A monument is a structure or construction of historical, cultural, or artistic significance, often built to commemorate an event or person."@en ;
          rdfs:label "Monument"@en .


###  http://www.semanticweb.org/usuario/ontologies/2025/3/Turismo_Inteligente_Recomendaciones#Museum
:Museum rdf:type owl:Class ;
        rdfs:subClassOf :Attraction ;
        rdfs:comment "A museum is a public space where art objects are displayed"@en ;
        rdfs:label "Museum"@en .


###  http://www.semanticweb.org/usuario/ontologies/2025/3/Turismo_Inteligente_Recomendaciones#MusicEvent
:MusicEvent rdf:type owl:Class ;
            rdfs:subClassOf :Event ;
            rdfs:comment "A music event is an event focused on the performance, enjoyment, or promotion of music, such as concerts, festivals, or recitals."@en ;
            rdfs:label "MusicEvent"@en .


###  http://www.semanticweb.org/usuario/ontologies/2025/3/Turismo_Inteligente_Recomendaciones#Park
:Park rdf:type owl:Class ;
      rdfs:subClassOf :Attraction ;
      rdfs:comment "A park is a public space with plants"@en ;
      rdfs:label "Park"@en .


###  http://www.semanticweb.org/usuario/ontologies/2025/3/Turismo_Inteligente_Recomendaciones#Price
:Price rdf:type owl:Class ;
       rdfs:comment "Indicates the cost associated with a product, service, or establishment.\""@en ;
       rdfs:label "Price"@en .


###  http://www.semanticweb.org/usuario/ontologies/2025/3/Turismo_Inteligente_Recomendaciones#Rating
:Rating rdf:type owl:Class ;
        rdfs:comment "Reflects the evaluation score given to a product, service, or establishment, typically based on user reviews or expert assessments."@en ;
        rdfs:label "Rating"@en .


###  http://www.semanticweb.org/usuario/ontologies/2025/3/Turismo_Inteligente_Recomendaciones#Restaurant
:Restaurant rdf:type owl:Class ;
            rdfs:subClassOf [ rdf:type owl:Restriction ;
                              owl:onProperty :isLocatedIn ;
                              owl:qualifiedCardinality "1"^^xsd:nonNegativeInteger ;
                              owl:onClass :City
                            ] ;
            rdfs:comment "An establishment where meals are prepared and served to customers."@en ;
            rdfs:label "Restaurant"@en .


###  http://www.semanticweb.org/usuario/ontologies/2025/3/Turismo_Inteligente_Recomendaciones#SportsEvent
:SportsEvent rdf:type owl:Class ;
             rdfs:subClassOf :Event ;
             rdfs:comment "A sports event is a competition, exhibition, or gathering organized around one or more sports disciplines."@en ;
             rdfs:label "SportsEvent"@en .


###  http://www.semanticweb.org/usuario/ontologies/2025/3/Turismo_Inteligente_Recomendaciones#Taxi
:Taxi rdf:type owl:Class ;
      rdfs:subClassOf :Transport .


###  http://www.semanticweb.org/usuario/ontologies/2025/3/Turismo_Inteligente_Recomendaciones#TechnologicEvent
:TechnologicEvent rdf:type owl:Class ;
                  rdfs:subClassOf :Event ;
                  rdfs:comment "A technological event is an event focused on technology, innovation, or scientific-technical development, such as fairs, conferences, or product launches."@en ;
                  rdfs:label "TechnologicalEvent"@en .


###  http://www.semanticweb.org/usuario/ontologies/2025/3/Turismo_Inteligente_Recomendaciones#TouristHotel
:TouristHotel rdf:type owl:Class ;
              rdfs:subClassOf :Hotel ;
              rdfs:comment "A tourist hotel is a hotel intended for general tourists, typically offering basic to moderate services at affordable prices."@en ;
              rdfs:label "TouristHotel"@en .


###  http://www.semanticweb.org/usuario/ontologies/2025/3/Turismo_Inteligente_Recomendaciones#Tram
:Tram rdf:type owl:Class ;
      rdfs:subClassOf :Transport ;
      rdfs:comment "A rail vehicle that runs on tracks laid in city streets, used for public urban transport"@en ;
      rdfs:label "Tram"@en .


###  http://www.semanticweb.org/usuario/ontologies/2025/3/Turismo_Inteligente_Recomendaciones#Transport
:Transport rdf:type owl:Class ;
           rdfs:comment "Means or systems used to move people or goods from one place to another"@en ;
           rdfs:label "Transport"@en .


#################################################################
#    Individuals
#################################################################

###  http://www.semanticweb.org/usuario/ontologies/2025/3/Turismo_Inteligente_Recomendaciones#Andaluza
:Andaluza rdf:type owl:NamedIndividual .


###  http://www.semanticweb.org/usuario/ontologies/2025/3/Turismo_Inteligente_Recomendaciones#Autobús
:Autobús rdf:type owl:NamedIndividual .


###  http://www.semanticweb.org/usuario/ontologies/2025/3/Turismo_Inteligente_Recomendaciones#Bicicleta
:Bicicleta rdf:type owl:NamedIndividual .


###  http://www.semanticweb.org/usuario/ontologies/2025/3/Turismo_Inteligente_Recomendaciones#Bilbao
:Bilbao rdf:type owl:NamedIndividual ,
                 :City ;
        :hasCityId 6 ;
        :hasCoordinates "43.2630,-2.9350" ;
        :name "Bilbao" .


###  http://www.semanticweb.org/usuario/ontologies/2025/3/Turismo_Inteligente_Recomendaciones#Congreso_Bilbao
:Congreso_Bilbao rdf:type owl:NamedIndividual ,
                          :CulturalEvent ;
                 :isLocatedIn :Bilbao ;
                 :hasDate "2024-12-01"^^xsd:date ;
                 :name "Congreso Bilbao" ;
                 rdfs:comment "A beach is a seaside tourist attraction." ;
                 rdfs:label "Beach"@en .


###  http://www.semanticweb.org/usuario/ontologies/2025/3/Turismo_Inteligente_Recomendaciones#CulturalAtraccion
:CulturalAtraccion rdf:type owl:NamedIndividual .


###  http://www.semanticweb.org/usuario/ontologies/2025/3/Turismo_Inteligente_Recomendaciones#CulturalEvento
:CulturalEvento rdf:type owl:NamedIndividual .


###  http://www.semanticweb.org/usuario/ontologies/2025/3/Turismo_Inteligente_Recomendaciones#Deportivo
:Deportivo rdf:type owl:NamedIndividual .


###  http://www.semanticweb.org/usuario/ontologies/2025/3/Turismo_Inteligente_Recomendaciones#Gastronómico
:Gastronómico rdf:type owl:NamedIndividual .


###  http://www.semanticweb.org/usuario/ontologies/2025/3/Turismo_Inteligente_Recomendaciones#Gourmet_Madrid
:Gourmet_Madrid rdf:type owl:NamedIndividual ,
                         :JapaneseRestaurant ;
                :hasPrice <http://www.semanticweb.org/usuario/ontologies/2025/3/Turismo_Inteligente_Recomendaciones#30> ;
                :hasRating :rating4_8 ;
                :isLocatedIn :Madrid ;
                :name "Restaurant Gourmet Madrid" .


###  http://www.semanticweb.org/usuario/ontologies/2025/3/Turismo_Inteligente_Recomendaciones#Italiana
:Italiana rdf:type owl:NamedIndividual .


###  http://www.semanticweb.org/usuario/ontologies/2025/3/Turismo_Inteligente_Recomendaciones#Japonesa
:Japonesa rdf:type owl:NamedIndividual .


###  http://www.semanticweb.org/usuario/ontologies/2025/3/Turismo_Inteligente_Recomendaciones#Lujo
:Lujo rdf:type owl:NamedIndividual .


###  http://www.semanticweb.org/usuario/ontologies/2025/3/Turismo_Inteligente_Recomendaciones#Madrid
:Madrid rdf:type owl:NamedIndividual ,
                 :City ;
        :hasAttraction :Museo_Madrid ;
        :hasHotel :Palace_Madrid ;
        :hasTransport :Urban_Madrid ;
        :hasCityId 3 ;
        :hasCoordinates "40.4168,-3.7038" ;
        :name "Madrid" .


###  http://www.semanticweb.org/usuario/ontologies/2025/3/Turismo_Inteligente_Recomendaciones#Mediterránea
:Mediterránea rdf:type owl:NamedIndividual .


###  http://www.semanticweb.org/usuario/ontologies/2025/3/Turismo_Inteligente_Recomendaciones#Metro
:Metro rdf:type owl:NamedIndividual .


###  http://www.semanticweb.org/usuario/ontologies/2025/3/Turismo_Inteligente_Recomendaciones#Mexicana
:Mexicana rdf:type owl:NamedIndividual .


###  http://www.semanticweb.org/usuario/ontologies/2025/3/Turismo_Inteligente_Recomendaciones#Monumento
:Monumento rdf:type owl:NamedIndividual .


###  http://www.semanticweb.org/usuario/ontologies/2025/3/Turismo_Inteligente_Recomendaciones#Museo
:Museo rdf:type owl:NamedIndividual .


###  http://www.semanticweb.org/usuario/ontologies/2025/3/Turismo_Inteligente_Recomendaciones#Museo_Madrid
:Museo_Madrid rdf:type owl:NamedIndividual ,
                       :Museum ;
              :hasRating :rating3_7 ;
              :isLocatedIn :Madrid ;
              :attraction_id 4 ;
              :name "Museo Madrid" .


###  http://www.semanticweb.org/usuario/ontologies/2025/3/Turismo_Inteligente_Recomendaciones#Música
:Música rdf:type owl:NamedIndividual .


###  http://www.semanticweb.org/usuario/ontologies/2025/3/Turismo_Inteligente_Recomendaciones#Negocios
:Negocios rdf:type owl:NamedIndividual .


###  http://www.semanticweb.org/usuario/ontologies/2025/3/Turismo_Inteligente_Recomendaciones#Palace_Madrid
:Palace_Madrid rdf:type owl:NamedIndividual ,
                        :LuxuryHotel ;
               :hasPrice <http://www.semanticweb.org/usuario/ontologies/2025/3/Turismo_Inteligente_Recomendaciones#227> ;
               :hasRating :rating5_0 ;
               :hasStars <http://www.semanticweb.org/usuario/ontologies/2025/3/Turismo_Inteligente_Recomendaciones#5Stars> ;
               :isLocatedIn :Madrid ;
               :hotel_id 42 ;
               :name "Hotel Palace Madrid" .


###  http://www.semanticweb.org/usuario/ontologies/2025/3/Turismo_Inteligente_Recomendaciones#Pamplona
:Pamplona rdf:type owl:NamedIndividual ,
                   :City .


###  http://www.semanticweb.org/usuario/ontologies/2025/3/Turismo_Inteligente_Recomendaciones#Parque
:Parque rdf:type owl:NamedIndividual .


###  http://www.semanticweb.org/usuario/ontologies/2025/3/Turismo_Inteligente_Recomendaciones#PlayaAtraccion
:PlayaAtraccion rdf:type owl:NamedIndividual .


###  http://www.semanticweb.org/usuario/ontologies/2025/3/Turismo_Inteligente_Recomendaciones#Royal_Pamplona
:Royal_Pamplona rdf:type owl:NamedIndividual ,
                         :LuxuryHotel ;
                :hasPrice <http://www.semanticweb.org/usuario/ontologies/2025/3/Turismo_Inteligente_Recomendaciones#116> ;
                :hasRating :rating4_3 ;
                :hasStars <http://www.semanticweb.org/usuario/ontologies/2025/3/Turismo_Inteligente_Recomendaciones#5Stars> ;
                :isLocatedIn :Pamplona ;
                :hotel_id 43 ;
                :name "Hotel Royal Pamplona" .


###  http://www.semanticweb.org/usuario/ontologies/2025/3/Turismo_Inteligente_Recomendaciones#Rural
:Rural rdf:type owl:NamedIndividual .


###  http://www.semanticweb.org/usuario/ontologies/2025/3/Turismo_Inteligente_Recomendaciones#Sabor_Sevilla
:Sabor_Sevilla rdf:type owl:NamedIndividual ,
                        :ItalianRestaurant ;
               :hasPrice <http://www.semanticweb.org/usuario/ontologies/2025/3/Turismo_Inteligente_Recomendaciones#72> ;
               :hasRating :rating4_1 ;
               :isLocatedIn :Sevilla ;
               :name "Restaurante Sabor Sevilla" ;
               :restaurant_id 6 .


###  http://www.semanticweb.org/usuario/ontologies/2025/3/Turismo_Inteligente_Recomendaciones#Sevilla
:Sevilla rdf:type owl:NamedIndividual ,
                  :City .


###  http://www.semanticweb.org/usuario/ontologies/2025/3/Turismo_Inteligente_Recomendaciones#Taxi
:Taxi rdf:type owl:NamedIndividual .


###  http://www.semanticweb.org/usuario/ontologies/2025/3/Turismo_Inteligente_Recomendaciones#Tecnológico
:Tecnológico rdf:type owl:NamedIndividual .


###  http://www.semanticweb.org/usuario/ontologies/2025/3/Turismo_Inteligente_Recomendaciones#Turistico
:Turistico rdf:type owl:NamedIndividual .


###  http://www.semanticweb.org/usuario/ontologies/2025/3/Turismo_Inteligente_Recomendaciones#Urban_Madrid
:Urban_Madrid rdf:type owl:NamedIndividual ,
                       :Metro ;
              :hasPrice <http://www.semanticweb.org/usuario/ontologies/2025/3/Turismo_Inteligente_Recomendaciones#8.85> ;
              :isLocatedIn :Madrid ;
              :name "Urban Madrid" ;
              :transport_id 1 .


###  http://www.semanticweb.org/usuario/ontologies/2025/3/Turismo_Inteligente_Recomendaciones#rating3_7
:rating3_7 rdf:type owl:NamedIndividual ,
                    :MediumRating ,
                    :Rating .


###  http://www.semanticweb.org/usuario/ontologies/2025/3/Turismo_Inteligente_Recomendaciones#rating3_9
:rating3_9 rdf:type owl:NamedIndividual ,
                    :MediumRating ,
                    :Rating .


###  http://www.semanticweb.org/usuario/ontologies/2025/3/Turismo_Inteligente_Recomendaciones#rating4_1
:rating4_1 rdf:type owl:NamedIndividual ,
                    :HighRating .


###  http://www.semanticweb.org/usuario/ontologies/2025/3/Turismo_Inteligente_Recomendaciones#rating4_3
:rating4_3 rdf:type owl:NamedIndividual ,
                    :HighRating .


###  http://www.semanticweb.org/usuario/ontologies/2025/3/Turismo_Inteligente_Recomendaciones#rating4_8
:rating4_8 rdf:type owl:NamedIndividual ,
                    :HighRating .


###  http://www.semanticweb.org/usuario/ontologies/2025/3/Turismo_Inteligente_Recomendaciones#rating5_0
:rating5_0 rdf:type owl:NamedIndividual ,
                    :HighRating .


###  http://www.semanticweb.org/usuario/ontologies/2025/3/Turismo_Inteligente_Recomendaciones#116
<http://www.semanticweb.org/usuario/ontologies/2025/3/Turismo_Inteligente_Recomendaciones#116> rdf:type owl:NamedIndividual ,
                                                                                                        :Price .


###  http://www.semanticweb.org/usuario/ontologies/2025/3/Turismo_Inteligente_Recomendaciones#227
<http://www.semanticweb.org/usuario/ontologies/2025/3/Turismo_Inteligente_Recomendaciones#227> rdf:type owl:NamedIndividual ,
                                                                                                        :Price .


###  http://www.semanticweb.org/usuario/ontologies/2025/3/Turismo_Inteligente_Recomendaciones#3Stars
<http://www.semanticweb.org/usuario/ontologies/2025/3/Turismo_Inteligente_Recomendaciones#3Stars> rdf:type owl:NamedIndividual ,
                                                                                                           :HotelStars .


###  http://www.semanticweb.org/usuario/ontologies/2025/3/Turismo_Inteligente_Recomendaciones#30
<http://www.semanticweb.org/usuario/ontologies/2025/3/Turismo_Inteligente_Recomendaciones#30> rdf:type owl:NamedIndividual ,
                                                                                                       :Price .


###  http://www.semanticweb.org/usuario/ontologies/2025/3/Turismo_Inteligente_Recomendaciones#5Stars
<http://www.semanticweb.org/usuario/ontologies/2025/3/Turismo_Inteligente_Recomendaciones#5Stars> rdf:type owl:NamedIndividual ,
                                                                                                           :HotelStars .


###  http://www.semanticweb.org/usuario/ontologies/2025/3/Turismo_Inteligente_Recomendaciones#56
<http://www.semanticweb.org/usuario/ontologies/2025/3/Turismo_Inteligente_Recomendaciones#56> rdf:type owl:NamedIndividual ,
                                                                                                       :Price ;
                                                                                              :hasRating :rating3_9 .


###  http://www.semanticweb.org/usuario/ontologies/2025/3/Turismo_Inteligente_Recomendaciones#72
<http://www.semanticweb.org/usuario/ontologies/2025/3/Turismo_Inteligente_Recomendaciones#72> rdf:type owl:NamedIndividual ,
                                                                                                       :Price .


###  http://www.semanticweb.org/usuario/ontologies/2025/3/Turismo_Inteligente_Recomendaciones#8.85
<http://www.semanticweb.org/usuario/ontologies/2025/3/Turismo_Inteligente_Recomendaciones#8.85> rdf:type owl:NamedIndividual ,
                                                                                                         :Price .


#################################################################
#    Annotations
#################################################################

:Metro rdfs:comment "An urban, high-capacity public transport system operating on an underground or elevated railway."@en ;
       rdfs:label "Metro"@en .


:Taxi rdfs:comment "A vehicle available for hire with a driver, offering point-to-point transport services"@en ;
      rdfs:label "Taxi"@en .


#################################################################
#    Rules
#################################################################

<http://www.semanticweb.org/usuario/ontologies/2025/3/Turismo_Inteligente_Recomendaciones/h> rdf:type <http://www.w3.org/2003/11/swrl#Variable> .

<http://www.semanticweb.org/usuario/ontologies/2025/3/Turismo_Inteligente_Recomendaciones/r> rdf:type <http://www.w3.org/2003/11/swrl#Variable> .

[ <http://swrl.stanford.edu/ontologies/3.3/swrla.owl#isRuleEnabled> "true"^^xsd:boolean ;
   rdfs:comment "If a hotel has a rating that is an instance of HighRating, then the hotel is a LuxuryHotel" ;
   rdfs:label "S1" ;
   rdf:type <http://www.w3.org/2003/11/swrl#Imp> ;
   <http://www.w3.org/2003/11/swrl#body> [ rdf:type <http://www.w3.org/2003/11/swrl#AtomList> ;
                                           rdf:first [ rdf:type <http://www.w3.org/2003/11/swrl#ClassAtom> ;
                                                       <http://www.w3.org/2003/11/swrl#classPredicate> :Hotel ;
                                                       <http://www.w3.org/2003/11/swrl#argument1> <http://www.semanticweb.org/usuario/ontologies/2025/3/Turismo_Inteligente_Recomendaciones/h>
                                                     ] ;
                                           rdf:rest [ rdf:type <http://www.w3.org/2003/11/swrl#AtomList> ;
                                                      rdf:first [ rdf:type <http://www.w3.org/2003/11/swrl#IndividualPropertyAtom> ;
                                                                  <http://www.w3.org/2003/11/swrl#propertyPredicate> :hasRating ;
                                                                  <http://www.w3.org/2003/11/swrl#argument1> <http://www.semanticweb.org/usuario/ontologies/2025/3/Turismo_Inteligente_Recomendaciones/h> ;
                                                                  <http://www.w3.org/2003/11/swrl#argument2> <http://www.semanticweb.org/usuario/ontologies/2025/3/Turismo_Inteligente_Recomendaciones/r>
                                                                ] ;
                                                      rdf:rest [ rdf:type <http://www.w3.org/2003/11/swrl#AtomList> ;
                                                                 rdf:first [ rdf:type <http://www.w3.org/2003/11/swrl#ClassAtom> ;
                                                                             <http://www.w3.org/2003/11/swrl#classPredicate> :HighRating ;
                                                                             <http://www.w3.org/2003/11/swrl#argument1> <http://www.semanticweb.org/usuario/ontologies/2025/3/Turismo_Inteligente_Recomendaciones/r>
                                                                           ] ;
                                                                 rdf:rest rdf:nil
                                                               ]
                                                    ]
                                         ] ;
   <http://www.w3.org/2003/11/swrl#head> [ rdf:type <http://www.w3.org/2003/11/swrl#AtomList> ;
                                           rdf:first [ rdf:type <http://www.w3.org/2003/11/swrl#ClassAtom> ;
                                                       <http://www.w3.org/2003/11/swrl#classPredicate> :LuxuryHotel ;
                                                       <http://www.w3.org/2003/11/swrl#argument1> <http://www.semanticweb.org/usuario/ontologies/2025/3/Turismo_Inteligente_Recomendaciones/h>
                                                     ] ;
                                           rdf:rest rdf:nil
                                         ]
 ] .

###  Generated by the OWL API (version 5.1.18) https://github.com/owlcs/owlapi/
